wip

src/riot/RIoT.Core.fst
@@ -27,9 +27,60 @@ open RIoT.Impl
 
 module Ed25519 = Hacl.Ed25519
 
-#set-options "--z3rlimit 50 --fuel 0 --ifuel 0 --admit_smt_queries true"
+#set-options "--z3rlimit 50 --fuel 0 --ifuel 0 --using_facts_from '* -FStar.Tactics -FStar.Reflection'"
 
-#restart-solver
+noeq
+type deviceIDCSR_ingredients_t = {
+  deviceIDCSR_ku: key_usage_payload_t;
+  deviceIDCSR_version: datatype_of_asn1_type INTEGER;
+  deviceIDCSR_s_common:  x509_RDN_x520_attribute_string_t COMMON_NAME  IA5_STRING;
+  deviceIDCSR_s_org:     x509_RDN_x520_attribute_string_t ORGANIZATION IA5_STRING;
+  deviceIDCSR_s_country: x509_RDN_x520_attribute_string_t COUNTRY      PRINTABLE_STRING
+}
+
+noeq
+type aliasKeyCRT_ingredients_t = {
+  aliasKeyCrt_version: x509_version_t;
+  aliasKeyCrt_serialNumber: x509_serialNumber_t;
+  aliasKeyCrt_i_common:  x509_RDN_x520_attribute_string_t COMMON_NAME  IA5_STRING;
+  aliasKeyCrt_i_org:     x509_RDN_x520_attribute_string_t ORGANIZATION IA5_STRING;
+  aliasKeyCrt_i_country: x509_RDN_x520_attribute_string_t COUNTRY      PRINTABLE_STRING;
+  aliasKeyCrt_notBefore: datatype_of_asn1_type Generalized_Time;
+  aliasKeyCrt_notAfter : datatype_of_asn1_type Generalized_Time;
+  aliasKeyCrt_s_common:  x509_RDN_x520_attribute_string_t COMMON_NAME  IA5_STRING;
+  aliasKeyCrt_s_org:     x509_RDN_x520_attribute_string_t ORGANIZATION IA5_STRING;
+  aliasKeyCrt_s_country: x509_RDN_x520_attribute_string_t COUNTRY      PRINTABLE_STRING;
+  aliasKeyCrt_ku: key_usage_payload_t;
+  aliasKeyCrt_riot_version: datatype_of_asn1_type INTEGER;
+}
+
+let deviceIDCRI_pre (x:deviceIDCSR_ingredients_t) =
+  valid_deviceIDCRI_ingredients
+    x.deviceIDCSR_version x.deviceIDCSR_s_common x.deviceIDCSR_s_org x.deviceIDCSR_s_country x.deviceIDCSR_ku
+
+[@@ "opaque_to_smt"]
+unfold noextract
+let coerce_asn1_tlv_int32_of_type_to_asn1_int32 (x:asn1_TLV_int32_of_type SEQUENCE)
+  : asn1_int32 = x
+
+let deviceIDCSR_pre (x:deviceIDCSR_ingredients_t{deviceIDCRI_pre x}) (deviceIDCSR_len:UInt32.t) =
+  let l = coerce_asn1_tlv_int32_of_type_to_asn1_int32
+    (len_of_deviceIDCRI
+      x.deviceIDCSR_version x.deviceIDCSR_s_common x.deviceIDCSR_s_org
+      x.deviceIDCSR_s_country x.deviceIDCSR_ku) in
+  
+  valid_deviceIDCSR_ingredients l /\
+  eq2 #nat (v deviceIDCSR_len) (length_of_deviceIDCSR l)
+
+let aliasKeyCRT_pre (x:aliasKeyCRT_ingredients_t) (aliasKeyCRT_len:UInt32.t) =
+  let l = coerce_asn1_tlv_int32_of_type_to_asn1_int32
+    (len_of_aliasKeyTBS
+      x.aliasKeyCrt_serialNumber x.aliasKeyCrt_i_common x.aliasKeyCrt_i_org x.aliasKeyCrt_i_country
+      x.aliasKeyCrt_s_common x.aliasKeyCrt_s_org x.aliasKeyCrt_s_country x.aliasKeyCrt_ku
+      x.aliasKeyCrt_riot_version) in
+  valid_aliasKeyCRT_ingredients l /\
+  eq2 #nat (v aliasKeyCRT_len) (length_of_aliasKeyCRT l)
+
 let riot_pre
   (h: HS.mem)
 (* Common Inputs *)
@@ -40,24 +91,9 @@ let riot_pre
   (aliasKey_label_len: size_t)
   (aliasKey_label: B.lbuffer byte_sec (v aliasKey_label_len))
 (* DeviceID CSR Inputs*)
-  (deviceIDCSR_ku: key_usage_payload_t)
-  (deviceIDCSR_version: datatype_of_asn1_type INTEGER)
-  (deviceIDCSR_s_common:  x509_RDN_x520_attribute_string_t COMMON_NAME  IA5_STRING)
-  (deviceIDCSR_s_org:     x509_RDN_x520_attribute_string_t ORGANIZATION IA5_STRING)
-  (deviceIDCSR_s_country: x509_RDN_x520_attribute_string_t COUNTRY      PRINTABLE_STRING)
+  (deviceIDCSR_ingredients:deviceIDCSR_ingredients_t)
 (* AliasKey Crt Inputs*)
-  (aliasKeyCrt_version: x509_version_t)
-  (aliasKeyCrt_serialNumber: x509_serialNumber_t)
-  (aliasKeyCrt_i_common:  x509_RDN_x520_attribute_string_t COMMON_NAME  IA5_STRING)
-  (aliasKeyCrt_i_org:     x509_RDN_x520_attribute_string_t ORGANIZATION IA5_STRING)
-  (aliasKeyCrt_i_country: x509_RDN_x520_attribute_string_t COUNTRY      PRINTABLE_STRING)
-  (aliasKeyCrt_notBefore: datatype_of_asn1_type Generalized_Time)
-  (aliasKeyCrt_notAfter : datatype_of_asn1_type Generalized_Time)
-  (aliasKeyCrt_s_common:  x509_RDN_x520_attribute_string_t COMMON_NAME  IA5_STRING)
-  (aliasKeyCrt_s_org:     x509_RDN_x520_attribute_string_t ORGANIZATION IA5_STRING)
-  (aliasKeyCrt_s_country: x509_RDN_x520_attribute_string_t COUNTRY      PRINTABLE_STRING)
-  (aliasKeyCrt_ku: key_usage_payload_t)
-  (riot_version: datatype_of_asn1_type INTEGER)
+  (aliasKeyCRT_ingredients:aliasKeyCRT_ingredients_t)
 (* Common Outputs *)
   (aliasKey_pub: B.lbuffer byte_pub 32)
   (aliasKey_priv: B.lbuffer uint8 32)
@@ -87,49 +123,65 @@ let riot_pre
    (* Pre: labels have enough length for HKDF *)
    valid_hkdf_lbl_len deviceID_label_len /\
    valid_hkdf_lbl_len aliasKey_label_len /\
-  // (let aliasKeyCrt_keyID_seq: lbytes_pub 20 =
-  //    derive_authKeyID_from_cdi_spec (B.as_seq h cdi) (deviceID_label_len) (B.as_seq h deviceID_label) in
-  //  let aliasKeyCrt_keyID = sha1_digest_to_octet_string_spec aliasKeyCrt_keyID_seq in
-   (* Pre: DeviceIDCRI template has a valid length *)
-   valid_deviceIDCRI_ingredients
-     deviceIDCSR_version
-     deviceIDCSR_s_common deviceIDCSR_s_org deviceIDCSR_s_country
-     deviceIDCSR_ku /\
-   (* Pre: DeviceIDCSR will have a valid length *)
-   valid_deviceIDCSR_ingredients
-     (len_of_deviceIDCRI
-       deviceIDCSR_version
-       deviceIDCSR_s_common deviceIDCSR_s_org deviceIDCSR_s_country
-       deviceIDCSR_ku) /\
-   (* Pre: `deviceIDCSR_buf` has exact size to write DeviceIDCSR *)
-   v deviceIDCSR_len == length_of_deviceIDCSR
-                          (len_of_deviceIDCRI
-                            deviceIDCSR_version
-                            deviceIDCSR_s_common deviceIDCSR_s_org deviceIDCSR_s_country
-                            deviceIDCSR_ku) /\
-   // (* Pre: AliasKeyTBS template has a valid length *)
-   // valid_aliasKeyTBS_ingredients
-   //   aliasKeyCrt_serialNumber
-   //   aliasKeyCrt_i_common aliasKeyCrt_i_org aliasKeyCrt_i_country
-   //   aliasKeyCrt_s_common aliasKeyCrt_s_org aliasKeyCrt_s_country
-   //   aliasKeyCrt_ku
-   //   riot_version /\
-   (* Pre: AliasKeyTBS will have a valid length *)
-   valid_aliasKeyCRT_ingredients
-     (len_of_aliasKeyTBS
-       aliasKeyCrt_serialNumber
-       aliasKeyCrt_i_common aliasKeyCrt_i_org aliasKeyCrt_i_country
-       aliasKeyCrt_s_common aliasKeyCrt_s_org aliasKeyCrt_s_country
-       aliasKeyCrt_ku
-       riot_version) /\
-   (* Pre: `aliasKeyCRT_buf` has exact size to write AliasKeyCRT *)
-   v aliasKeyCRT_len == length_of_aliasKeyCRT
-                          (len_of_aliasKeyTBS
-                            aliasKeyCrt_serialNumber
-                            aliasKeyCrt_i_common aliasKeyCrt_i_org aliasKeyCrt_i_country
-                            aliasKeyCrt_s_common aliasKeyCrt_s_org aliasKeyCrt_s_country
-                            aliasKeyCrt_ku
-                            riot_version)
+
+   deviceIDCRI_pre deviceIDCSR_ingredients /\
+   deviceIDCSR_pre deviceIDCSR_ingredients deviceIDCSR_len /\
+   aliasKeyCRT_pre aliasKeyCRT_ingredients aliasKeyCRT_len
+
+let aliasKey_post
+  (cdi : B.lbuffer byte_sec 32) (fwid: B.lbuffer byte_sec 32)
+  (aliasKey_label_len:UInt32.t{valid_hkdf_lbl_len aliasKey_label_len})
+  (aliasKey_label: B.lbuffer byte_sec (v aliasKey_label_len))
+  (aliasKey_pub: B.lbuffer byte_pub 32)
+  (aliasKey_priv: B.lbuffer uint8 32)
+  (h0 h1:HS.mem)
+ = ((B.as_seq h1 aliasKey_pub  <: lbytes_pub 32),
+    (B.as_seq h1 aliasKey_priv <: lbytes_sec 32)) == derive_AliasKey_spec
+                                                       (B.as_seq h0 cdi)
+                                                       (B.as_seq h0 fwid)
+                                                       aliasKey_label_len
+                                                       (B.as_seq h0 aliasKey_label)
+
+#push-options "--z3rlimit 100"
+let deviceIDCSR_post
+  (cdi:B.lbuffer byte_sec 32)
+  (deviceID_label_len:UInt32.t{valid_hkdf_lbl_len deviceID_label_len})
+  (deviceID_label:B.lbuffer byte_sec (v deviceID_label_len))
+  (deviceIDCSR_ingredients:deviceIDCSR_ingredients_t{
+    valid_deviceIDCRI_ingredients
+      deviceIDCSR_ingredients.deviceIDCSR_version deviceIDCSR_ingredients.deviceIDCSR_s_common
+      deviceIDCSR_ingredients.deviceIDCSR_s_org deviceIDCSR_ingredients.deviceIDCSR_s_country
+      deviceIDCSR_ingredients.deviceIDCSR_ku})
+  (deviceIDCSR_len:UInt32.t)
+  (deviceIDCSR_buf:B.lbuffer byte_pub (v deviceIDCSR_len))
+  (h0 h1:HS.mem)
+  = let deviceID_pub_seq, deviceID_priv_seq = derive_DeviceID_spec
+                                                (B.as_seq h0 cdi)
+                                                (deviceID_label_len)
+                                                (B.as_seq h0 deviceID_label) in
+    let deviceIDCRI: deviceIDCRI_t = create_deviceIDCRI_spec
+      deviceIDCSR_ingredients.deviceIDCSR_version deviceIDCSR_ingredients.deviceIDCSR_s_common
+      deviceIDCSR_ingredients.deviceIDCSR_s_org deviceIDCSR_ingredients.deviceIDCSR_s_country
+      deviceIDCSR_ingredients.deviceIDCSR_ku deviceID_pub_seq in
+
+    let deviceIDCRI_seq = serialize_deviceIDCRI `serialize` deviceIDCRI in
+    
+    let deviceIDCRI_len = coerce_asn1_tlv_int32_of_type_to_asn1_int32
+      (len_of_deviceIDCRI
+        deviceIDCSR_ingredients.deviceIDCSR_version deviceIDCSR_ingredients.deviceIDCSR_s_common
+        deviceIDCSR_ingredients.deviceIDCSR_s_org deviceIDCSR_ingredients.deviceIDCSR_s_country
+        deviceIDCSR_ingredients.deviceIDCSR_ku) in
+      
+    let (* Prf *) _ = lemma_serialize_deviceIDCRI_size_exact deviceIDCRI in  //AR: TODO: This takes long time
+    assume (valid_deviceIDCSR_ingredients deviceIDCRI_len);  //AR: TODO: should come from pre, add to refinement
+    let deviceIDCSR: deviceIDCSR_t deviceIDCRI_len = sign_and_finalize_deviceIDCSR_spec
+                                                                (deviceID_priv_seq)
+                                                                (deviceIDCRI_len)
+                                                                (deviceIDCRI_seq) in
+    B.as_seq h1 deviceIDCSR_buf == serialize_deviceIDCSR deviceIDCRI_len `serialize` deviceIDCSR
+#pop-options
+
+#set-options "--admit_smt_queries true"  //AR: TODO: until here
 
 #restart-solver
 let riot_post
@@ -198,12 +250,7 @@ let riot_post
                   loc_buffer aliasKey_pub    `loc_union`
                   loc_buffer aliasKey_priv ) h0 h1) /\
     (* Post: AliasKey *)
-    ((B.as_seq h1 aliasKey_pub  <: lbytes_pub 32),
-     (B.as_seq h1 aliasKey_priv <: lbytes_sec 32)) == derive_AliasKey_spec
-                                                        (B.as_seq h0 cdi)
-                                                        (B.as_seq h0 fwid)
-                                                        aliasKey_label_len
-                                                        (B.as_seq h0 aliasKey_label) /\
+    aliasKey_post cdi fwid aliasKey_label_len aliasKey_label aliasKey_pub aliasKey_priv h0 h1 /\
     (* Post: AliasKeyCRT *)
     (let deviceID_pub_seq, deviceID_priv_seq = derive_DeviceID_spec
                                                  (B.as_seq h0 cdi)
